Factored out expression types

call_by_need.v
@@ -1,36 +1,8 @@
 (* Based on figure 8 of ariola et al *) 
 Require Import Lists.List.
 Require Import Unicode.Utf8_core.
-
-Definition id : Type := nat.
-
-Theorem eq_nat_dec : forall n m : id, {n = m} + {n <> m}.
-Proof.
-  (* WORKED IN CLASS *)
-  intros n.
-  induction n as [|n'].
-    intros m.
-    destruct m as [|m'].
-      left. reflexivity.
-      right. intros contra. inversion contra.
-    intros m.
-    destruct m as [|m'].
-      right. intros contra. inversion contra.
-      destruct IHn' with (m := m') as [eq | neq].
-      left. apply f_equal.  apply eq.
-      right. intros Heq. inversion Heq as [Heq']. apply neq. apply Heq'.
-Defined. 
-
-Inductive tm : Type :=
-  | var : id -> tm
-  | app : tm -> tm -> tm
-  | abs : id -> tm -> tm.
-
-Definition value (t : tm) : Prop := match t with
-  | abs _ _ => True
-  | _ => False
-  end.
-
+Require Import expr.
+Require Import Arith.Peano_dec.
 
 Definition heap := list (id * tm). 
 
@@ -45,20 +17,16 @@ Proof. simpl. right. left. reflexivity. Qed.
 Inductive configuration : Type := 
   | st : heap -> tm -> configuration.
 
-Notation " :λ x , N " := (abs x N) (at level 20).
-Notation " M @ N " := (app M N) (at level 60). 
-Coercion var : id >-> tm.
-
 Notation " x ↦ M " := (x, M) (at level 40).
 Notation " ⟨ Φ ⟩ m " := (st Φ m) (at level 40).
 Notation " ⟨ Ψ , b ⟩ N " := (st (cons b Ψ) N) (at level 40).
 Notation " ⟨ Φ , b , Ψ ⟩ N " := (st (Datatypes.app Ψ (cons b Φ)) N) (at level 40).
 
 Reserved Notation "'[' x '//' y ']' t" (at level 20).
-Fixpoint subst (x y : id) (t : tm) : tm := match t with
-  | var z => if eq_nat_dec z x then y else t
-  | m@n => [x//y]m @ [x//y]n
-  | :λy,b => if eq_nat_dec y x then t else (:λy,[x//y]b)
+Fixpoint subst (x x' : id) (t : tm) : tm := match t with
+  | var y => if eq_nat_dec y x then x else t
+  | m@n => [x'//x]m @ [x'//x]n
+  | :λy,b => if eq_nat_dec y x then t else (:λy,[x'//x]b)
   end
 where " '[' x '//' y ']' t " := (subst y x t).
 
@@ -68,16 +36,18 @@ Inductive step : configuration -> configuration -> Prop :=
   | Id : ∀ M N y x Φ Ψ Υ, ⟨Φ⟩M ⇓ ⟨Ψ⟩:λy,N ->
           ⟨Φ, x ↦ M, Υ⟩x ⇓ ⟨Ψ, x ↦ :λy,N, Υ⟩:λy,N
   | Abs : ∀ N x Φ, ⟨Φ⟩:λx,N ⇓ ⟨Φ⟩:λx,N
-  | App : ∀ M N L y x x' Φ Ψ Υ,⟨Φ⟩L ⇓ ⟨Ψ⟩:λx,N ->
-        ⟨Ψ, x' ↦ M⟩[x'//x]N ⇓ ⟨Υ⟩:λy,N ->
-           ⟨Φ⟩(L@M) ⇓ ⟨Υ⟩:λy,N
+  | App : ∀ M N L B y x x' Φ Ψ Υ,⟨Φ⟩L ⇓ ⟨Ψ⟩:λx,N ->
+        ⟨Ψ, x' ↦ M⟩[x'//x]N ⇓ ⟨Υ⟩:λy,B ->
+           ⟨Φ⟩(L@M) ⇓ ⟨Υ⟩:λy,B
 where " c1 '⇓' c2 " := (step c1 c2).
 
 Lemma values_only : ∀ c M Ψ, c ⇓ ⟨Ψ⟩M -> value M.
 intros. inversion H; simpl; auto. Qed. 
 
-Example simple (x :id) : (step (⟨nil⟩ app (abs x x) (abs x x)) (⟨nil, x ↦ :λx,x⟩ abs x x)).
-apply App with x x nil. apply Abs. simpl. destruct eq_nat_dec. rewrite <-
-app_nil_l with (prod id tm) (cons (x↦:λx,x) nil). apply Id. apply Abs. unfold
-not in n. assert (x = x). reflexivity. apply n in H. inversion H. Qed. 
+Example simple (x y :id) : (step (⟨nil⟩ ((:λx,x) @ (:λy,y))) (⟨nil, x ↦ :λy,y⟩ :λy, y)).
+apply App with x x x nil. apply Abs. simpl. destruct eq_nat_dec. rewrite <-
+app_nil_l with (prod id tm) (cons (x↦:λy,y) nil). rewrite <- app_nil_l with
+(prod id tm) (cons (x↦:λy,y) nil). apply Id. apply Abs. unfold not in n.
+assert (x = x). reflexivity. apply n in H. inversion H. Qed. 
+
 
