expr.v
@@ -1,0 +1,17 @@
+
+Definition id : Type := nat.
+
+Inductive tm : Type :=
+  | var : id -> tm
+  | app : tm -> tm -> tm
+  | abs : id -> tm -> tm.
+
+Definition value (t : tm) : Prop := match t with
+  | abs _ _ => True
+  | _ => False
+  end.
+
+Notation " :λ x , N " := (abs x N) (at level 20).
+Notation " M @ N " := (app M N) (at level 60). 
+Coercion var : id >-> tm.
+
