expr_db.v
@@ -1,0 +1,10 @@
+Require Vector.
+
+Inductive expr (n : nat) : Type := 
+  | var : Fin.t n -> expr n
+  | lam : expr (S n) -> expr n
+  | app : expr n -> expr n -> expr n.
+
+Example term_1 : expr 0 := lam 0 (var 1 Fin.F1).
+Example term_2 : expr 0 := app 0 term_1 term_1.
+
